src/mem/FiniteMaps.v
@@ -1,0 +1,52 @@
+From Coq Require Import
+  FSets.FMapAVL
+  FSets.FSetAVL
+  FSetProperties
+  FMapFacts.
+
+Module IM := FMapAVL.Make(Coq.Structures.OrderedTypeEx.Z_as_OT).
+Module IS := FSetAVL.Make(Coq.Structures.OrderedTypeEx.Z_as_OT).
+Module Import ISP := FSetProperties.WProperties_fun(Coq.Structures.OrderedTypeEx.Z_as_OT)(IS).
+Module Import IP := FMapFacts.WProperties_fun(Coq.Structures.OrderedTypeEx.Z_as_OT)(IM).
+
+Lemma find_add_eq :
+  forall {elt} (m : @IM.t elt) (k : IM.key) (v : elt),
+    IM.find k (IM.add k v m) = Some v.
+Proof.
+  intros elt m k v.
+  apply IM.find_1.
+  apply IM.add_1; auto.
+Qed.
+
+Lemma find_add_neq :
+  forall {elt} (m : @IM.t elt) (k1 k2 : IM.key) (v x : elt),
+    k1 <> k2 ->
+    IM.find k1 m = Some x ->
+    IM.find k1 (IM.add k2 v m) = Some x.
+Proof.
+  intros elt m k1 k2 v x NEQ FIND.
+  apply IM.find_1.
+  apply IM.add_2; auto.
+  apply IM.find_2; auto.
+Qed.
+
+Lemma IS_mem_add_eq :
+  forall (m : IS.t) (k : IS.elt),
+    IS.mem k (IS.add k m) = true.
+Proof.
+  intros m k.
+  apply IS.mem_1.
+  apply IS.add_1; auto.
+Qed.
+
+Lemma IS_mem_add_neq :
+  forall (m : IS.t) (k1 k2 : IS.elt),
+    k1 <> k2 ->
+    IS.mem k1 m = true ->
+    IS.mem k1 (IS.add k2 m) = true.
+Proof.
+  intros m k1 k2 NEQ IN.
+  apply IS.mem_1.
+  apply IS.add_2; auto.
+  apply IS.mem_2; auto.
+Qed.
